formatting

Cslib/Languages/LambdaCalculus/Named/Untyped/Basic.lean
@@ -14,7 +14,7 @@ public import Cslib.Foundations.Syntax.HasSubstitution
 
 /-! # λ-calculus
 
-The untyped λ-calculus.
+The untyped λ-calculus, with a named representation of variables.
 
 ## References
 
@@ -28,9 +28,9 @@ namespace Cslib
 
 universe u
 
-variable {Var : Type u}
+variable {Var : Type u} [DecidableEq Var] [HasFresh Var]
 
-namespace LambdaCalculus.Named
+namespace LambdaCalculus.Named.Untyped
 
 /-- Syntax of terms. -/
 inductive Term (Var : Type u) : Type u where
@@ -39,58 +39,59 @@ inductive Term (Var : Type u) : Type u where
   | app (m n : Term Var)
 deriving DecidableEq
 
+namespace Term
+
 /-- Free variables. -/
-def Term.fv [DecidableEq Var] : Term Var → Finset Var
+def fv : Term Var → Finset Var
   | var x => {x}
   | abs x m => m.fv \ {x}
   | app m n => m.fv ∪ n.fv
 
 /-- Bound variables. -/
-def Term.bv [DecidableEq Var] : Term Var → Finset Var
+def bv : Term Var → Finset Var
   | var _ => ∅
   | abs x m => m.bv ∪ {x}
   | app m n => m.bv ∪ n.bv
 
 /-- Variable names (free and bound) in a term. -/
-def Term.vars [DecidableEq Var] : Term Var → Finset Var
+def vars : Term Var → Finset Var
   | var x => {x}
   | abs x m => m.vars ∪ {x}
   | app m n => m.vars ∪ n.vars
 
 /-- Variable renaming, applying to both free and bound variables.
     `m.rename x y` changes all occurrences of `x` into `y` in `m`. -/
-def Term.rename [DecidableEq Var] (m : Term Var) (x y : Var) : Term Var :=
+def rename (m : Term Var) (x y : Var) : Term Var :=
   match m with
   | var z => var (if z = x then y else z)
   | abs z m' => abs (if z = x then y else z) (m'.rename x y)
   | app n1 n2 => app (n1.rename x y) (n2.rename x y)
 
+omit [HasFresh Var] in
 /-- Renaming preserves size. -/
 @[simp]
-theorem Term.rename.eq_sizeOf {m : Term Var} {x y : Var} [DecidableEq Var] :
-  sizeOf (m.rename x y) = sizeOf m := by
+theorem rename_eq_sizeOf {m : Term Var} {x y : Var} : sizeOf (m.rename x y) = sizeOf m := by
   induction m <;> aesop (add simp [Term.rename])
 
-open Term
-
 /-- α-equivalence. -/
-inductive Term.AlphaEquiv [DecidableEq Var] : Term Var → Term Var → Prop where
-| var {x} : AlphaEquiv (var x) (var x)
-| abs {y x1 x2 m1 m2} : y ∉ m1.vars ∪ m2.vars ∪ {x1, x2} →
-  AlphaEquiv (m1.rename x1 y) (m2.rename x2 y) → AlphaEquiv (abs x1 m1) (abs x2 m2)
-| app {m1 n1 m2 n2} : AlphaEquiv m1 n1 → AlphaEquiv m2 n2 → AlphaEquiv (app m1 m2) (app n1 n2)
+inductive AlphaEquiv : Term Var → Term Var → Prop where
+  | var {x} : AlphaEquiv (var x) (var x)
+  | abs {y x1 x2 m1 m2} : y ∉ m1.vars ∪ m2.vars ∪ {x1, x2} →
+    AlphaEquiv (m1.rename x1 y) (m2.rename x2 y) → AlphaEquiv (abs x1 m1) (abs x2 m2)
+  | app {m1 n1 m2 n2} : AlphaEquiv m1 n1 → AlphaEquiv m2 n2 → AlphaEquiv (app m1 m2) (app n1 n2)
 
 /-- Instance for the notation `m =α n`. -/
-instance instHasAlphaEquivTerm [DecidableEq Var] : HasAlphaEquiv (Term Var) where
-  AlphaEquiv := Term.AlphaEquiv
+instance instHasAlphaEquivTerm : HasAlphaEquiv (Term Var) where
+  AlphaEquiv := AlphaEquiv
 
+omit [HasFresh Var] in
 /-- Allow grind to recognise the notation of α-equivalence. -/
 @[grind ←]
-theorem Term.AlphaEquiv_def [DecidableEq Var] (m n : Term Var) :
-  AlphaEquiv m n ↔ m =α n := by rfl
+theorem AlphaEquiv_def (m n : Term Var) : AlphaEquiv m n ↔ m =α n := by
+  rfl
 
 /-- Capture-avoiding substitution, as an inference system. -/
-inductive Term.Subst [DecidableEq Var] : Term Var → Var → Term Var → Term Var → Prop where
+inductive Subst : Term Var → Var → Term Var → Term Var → Prop where
   | varHit {x r} : (var x).Subst x r r
   | varMiss {x y r} : y ≠ x → (var y).Subst x r (var y)
   | absShadow {x m r} : (abs x m).Subst x r (abs x m)
@@ -101,8 +102,8 @@ inductive Term.Subst [DecidableEq Var] : Term Var → Var → Term Var → Term 
 /-- Capture-avoiding substitution. `m.subst x r` replaces the free occurrences of variable `x`
 in `m` with `r`. -/
 @[grind, simp]
-def Term.subst [DecidableEq Var] [HasFresh Var] (m : Term Var) (x : Var) (r : Term Var) :
-  Term Var :=
+def subst (m : Term Var) (x : Var) (r : Term Var) :
+    Term Var :=
   match m with
   | var y => if y = x then r else var y
   | abs y m' =>
@@ -115,17 +116,17 @@ def Term.subst [DecidableEq Var] [HasFresh Var] (m : Term Var) (x : Var) (r : Te
       abs z ((m'.rename y z).subst x r)
   | app m1 m2 => app (m1.subst x r) (m2.subst x r)
 termination_by m
-decreasing_by all_goals grind [rename.eq_sizeOf, abs.sizeOf_spec, app.sizeOf_spec]
+decreasing_by all_goals grind [rename_eq_sizeOf, abs.sizeOf_spec, app.sizeOf_spec]
 
 /-- `Term.subst` is a substitution for λ-terms. Gives access to the notation `m[x := n]`. -/
-instance instHasSubstitutionTerm [DecidableEq Var] [HasFresh Var] :
+instance instHasSubstitutionTerm :
     HasSubstitution (Term Var) Var (Term Var) where
-  subst := Term.subst
+  subst := subst
 
 /-- Allow grind to recognise the notation of substitution. -/
 @[grind ←, simp← ]
-theorem Term.subst_def [DecidableEq Var] (m r : Term Var) (x : Var) [HasFresh Var] :
-  m.subst x r = m[x := r] := by rfl
+theorem subst_def (m r : Term Var) (x : Var) : m.subst x r = m[x := r] := by
+  rfl
 
 /-- Contexts. -/
 inductive Context (Var : Type u) : Type u where
@@ -143,12 +144,12 @@ def Context.fill (c : Context Var) (m : Term Var) : Term Var :=
   | appL c n => Term.app (c.fill m) n
   | appR n c => Term.app n (c.fill m)
 
-def Context.vars [DecidableEq Var] : Context Var → Finset Var
+def Context.vars : Context Var → Finset Var
   | hole => ∅
   | abs x c => c.vars ∪ {x}
   | appL c m => c.vars ∪ m.vars
   | appR m c => m.vars ∪ c.vars
 
-end LambdaCalculus.Named
+end LambdaCalculus.Named.Untyped.Term
 
 end Cslib
